theories/language/language.v
@@ -50,37 +50,19 @@ Proof.
   { destruct k; simpl; apply fill_not_val; done. }
   simplify_eq.
 Qed.
-Lemma prim_step_to_val_is_base_step e σ1 κ v σ2 es ϕ :
-  prim_step e σ1 κ (Val v) σ2 es ϕ →
-  base_step e σ1 κ (Val v) σ2 es ϕ.
+Lemma prim_step_to_val_is_base_step e σ1 κ v σ2 es :
+  prim_step e σ1 κ (Val v) σ2 es →
+  base_step e σ1 κ (Val v) σ2 es.
 Proof.
   intro H. destruct H as [K e1 e2 H1 H2].
   assert (to_val (fill K e2) = Some v) as H3; first rewrite -H2 //.
   apply to_val_fill_some in H3 as [-> ->]. subst e. done.
 Qed.
-Lemma base_step_to_val e σ1 κ1 e1 σ1' es1 ϕ1 σ2 κ2 e2 σ2' es2 ϕ2 :
-  base_step e σ1 κ1 e1 σ1' es1 ϕ1 →
-  base_step e σ2 κ2 e2 σ2' es2 ϕ2 →
+Lemma base_step_to_val e σ1 κ1 e1 σ1' es1 σ2 κ2 e2 σ2' es2 :
+  base_step e σ1 κ1 e1 σ1' es1 →
+  base_step e σ2 κ2 e2 σ2' es2 →
   is_Some (to_val e1) →
   is_Some (to_val e2).
 Proof.
   destruct 1; inversion 1; naive_solver.
-Qed.
-
-Lemma irreducible_resolve e v1 v2 σ :
-  irreducible e σ →
-  irreducible (Resolve e (Val v1) (Val v2)) σ.
-Proof.
-  intros H κ ? σ' es ϕ [K' e1' e2' Hfill -> step]. simpl in *.
-  induction K' as [| K K' _] using rev_ind; simpl in Hfill.
-  - subst e1'. inversion step. eapply H. apply base_prim_step. done.
-  - rewrite fill_app /= in Hfill.
-    destruct K;
-      inversion Hfill; subst; clear Hfill;
-      try match goal with H : Val ?v = fill K' ?e |- _ =>
-        assert (to_val (fill K' e) = Some v) as HEq by rewrite -H //;
-        apply to_val_fill_some in HEq; destruct HEq as [-> ->]; inversion step
-      end.
-    eapply (H κ (fill_item _ (foldl (flip fill_item) e2' K')) σ' es).
-    eapply (Ectx_step (K' ++ [_])); last done; simpl; rewrite fill_app //.
 Qed.
