theories/language/metatheory.v
@@ -43,8 +43,6 @@ Fixpoint occurs x e :=
         bool_decide (BNamed x ≠ pat.(pattern_as)) &&
         occurs x br.2
       ) brs
-  | Reveal e =>
-      occurs x e
   | For e1 e2 e3 =>
       occurs x e1 ||
       occurs x e2 ||
@@ -73,12 +71,6 @@ Fixpoint occurs x e :=
       occurs x e
   | Yield =>
       false
-  | Proph =>
-      false
-  | Resolve e0 e1 e2 =>
-      occurs x e0 ||
-      occurs x e1 ||
-      occurs x e2
   end.
 
 Definition val_recursive v :=
