theories/language/rules.v
@@ -16,7 +16,6 @@ From zoo Require Import
   options.
 
 Implicit Types l : location.
-Implicit Types pid : prophet_id.
 Implicit Types lit : literal.
 Implicit Types e : expr.
 Implicit Types es : list expr.
@@ -28,50 +27,43 @@ Section zoo_G.
   Context `{zoo_G : !ZooG Σ}.
 
   Lemma base_reducible_equal v1 v2 σ :
-    val_physical v1 →
-    val_physical v2 →
     base_reducible (v1 = v2) σ.
   Proof.
     destruct
-      v1 as [[b1 | i1 | l1 | |] | | [cid1 |] tag1 []],
-      v2 as [[b2 | i2 | l2 | |] | | [cid2 |] tag2 []].
+      v1 as [[b1 | i1 | l1] | | tag1 []],
+      v2 as [[b2 | i2 | l2] | | tag2 []].
     all:
       try first
       [ destruct (decide (b1 = b2)); first subst
       | destruct (decide (i1 = i2)); first subst
       | destruct (decide (l1 = l2)); first subst
-      | destruct (decide (cid1 = cid2)); first subst
       | destruct (decide (tag1 = tag2)); first subst
       ].
     all: auto with zoo.
   Qed.
   Lemma wp_equal v1 v2 E Φ :
-    val_physical v1 →
-    val_physical v2 →
     ▷ (
       ( ⌜val_neq v1 v2⌝ -∗
         Φ #false
       ) ∧ (
         ⌜val_eq v1 v2⌝ -∗
-        ⌜val_consistency v1 v2⌝ -∗
         Φ #true
       )
     ) ⊢
     WP v1 = v2 @ E {{ Φ }}.
   Proof.
-    iIntros "% % HΦ".
-    iApply wp_lift_atomic_base_step_no_fork; first done. iIntros "%nt %σ1 %κ %κs (Hσ & Hκs) !>".
+    iIntros "HΦ".
+    iApply wp_lift_atomic_base_step_no_fork; first done. iIntros "%nt %σ1 %κ %κs Hσ !>".
     iSplit. { iPureIntro. apply base_reducible_equal; done. }
-    iIntros "%e2 %σ2 %es %ϕ %Hstep %Hϕ _ !> !> !>".
+    iIntros "%e2 %σ2 %es %Hstep _ !> !> !>".
     destruct
-      v1 as [[b1 | i1 | l1 | |] | | [cid1 |] tag1 []],
-      v2 as [[b2 | i2 | l2 | |] | | [cid2 |] tag2 []].
+      v1 as [[b1 | i1 | l1] | | tag1 []],
+      v2 as [[b2 | i2 | l2] | | tag2 []].
     all:
       try first
       [ destruct (decide (b1 = b2)); first subst
       | destruct (decide (i1 = i2)); first subst
       | destruct (decide (l1 = l2)); first subst
-      | destruct (decide (cid1 = cid2)); first subst
       | destruct (decide (tag1 = tag2)); first subst
       ].
     all: invert_base_step; last try by exfalso.
@@ -86,19 +78,6 @@ Section zoo_G.
             iFrame; iSteps; naive_solver
         end
       end.
-  Qed.
-
-  Lemma wp_reveal tag vs E Φ :
-    ( ∀ cid,
-      ▷ Φ (ValConstr (Some cid) tag vs)
-    ) ⊢
-    WP Reveal $ ValConstr None tag vs @ E {{ Φ }}.
-  Proof.
-    iIntros "H".
-    iApply wp_lift_atomic_base_step_no_fork; first done. iIntros "%nt %σ1 %κ %κs (Hσ & Hκs) !>".
-    iSplit; first eauto with zoo. iIntros "%e2 %σ2 %es %ϕ %Hstep %Hϕ _ !> !> !>".
-    invert_base_step.
-    iFrame. iSteps.
   Qed.
 
   Lemma big_sepM_heap_array (Φ : location → val → iProp Σ) l vs :
@@ -127,8 +106,8 @@ Section zoo_G.
     }}}.
   Proof.
     iIntros (Hlen <-%of_to_vals) "%Φ _ HΦ".
-    iApply wp_lift_atomic_base_step_no_fork; first done. iIntros "%nt %σ1 %κ %κs (Hσ1 & Hκs) !>".
-    iSplit; first auto with zoo. iIntros "%e2 %σ2 %es %ϕ %Hstep %Hϕ _ !> !>".
+    iApply wp_lift_atomic_base_step_no_fork; first done. iIntros "%nt %σ1 %κ %κs Hσ1 !>".
+    iSplit; first auto with zoo. iIntros "%e2 %σ2 %es %Hstep _ !> !>".
     invert_base_step. rename select (list val) into vs.
     iStep. iFrame.
     iMod (gen_heap_alloc_big _ (heap_array _ _) with "Hσ1") as "($ & Hl & Hmeta)".
@@ -150,8 +129,8 @@ Section zoo_G.
     }}}.
   Proof.
     iIntros "%Hn %Φ _ HΦ".
-    iApply wp_lift_atomic_base_step_no_fork; first done. iIntros "%nt %σ1 %κ %κs (Hσ1 & Hκs) !>".
-    iSplit; first auto with zoo. iIntros "%e2 %σ2 %es %ϕ %Hstep %Hϕ _ !> !>".
+    iApply wp_lift_atomic_base_step_no_fork; first done. iIntros "%nt %σ1 %κ %κs Hσ1 !>".
+    iSplit; first auto with zoo. iIntros "%e2 %σ2 %es %Hstep _ !> !>".
     invert_base_step.
     iStep. iFrame.
     iMod (gen_heap_alloc_big _ (heap_array _ _) with "Hσ1") as "($ & Hl & Hmeta)".
@@ -186,9 +165,9 @@ Section zoo_G.
     }}}.
   Proof.
     iIntros "%Φ >Hl HΦ".
-    iApply wp_lift_atomic_base_step_no_fork; first done. iIntros "%nt %σ1 %κ %κs (Hσ & Hκs) !>".
+    iApply wp_lift_atomic_base_step_no_fork; first done. iIntros "%nt %σ1 %κ %κs Hσ !>".
     iDestruct (gen_heap_valid with "Hσ Hl") as %Hlookup.
-    iSplit; first eauto with zoo. iIntros "%e2 %σ2 %es %ϕ %Hstep %Hϕ _ !> !> !>".
+    iSplit; first eauto with zoo. iIntros "%e2 %σ2 %es %Hstep _ !> !> !>".
     invert_base_step.
     iFrame. iSteps.
   Qed.
@@ -204,9 +183,9 @@ Section zoo_G.
     }}}.
   Proof.
     iIntros "%Φ >Hl HΦ".
-    iApply wp_lift_atomic_base_step_no_fork; first done. iIntros "%nt %σ1 %κ %κs (Hσ & Hκs) !>".
+    iApply wp_lift_atomic_base_step_no_fork; first done. iIntros "%nt %σ1 %κ %κs Hσ !>".
     iDestruct (gen_heap_valid with "Hσ Hl") as %Hlookup.
-    iSplit; first eauto with zoo. iIntros "%e2 %σ2 %es %ϕ %Hstep %Hϕ _ !> !>".
+    iSplit; first eauto with zoo. iIntros "%e2 %σ2 %es %Hstep _ !> !>".
     invert_base_step.
     iMod (gen_heap_update with "Hσ Hl") as "($ & Hl)".
     iFrame. iSteps.
@@ -223,9 +202,9 @@ Section zoo_G.
     }}}.
   Proof.
     iIntros "%Φ >Hl HΦ".
-    iApply wp_lift_atomic_base_step_no_fork; first done. iIntros "%nt %σ1 %κ %κs (Hσ & Hκs) !>".
+    iApply wp_lift_atomic_base_step_no_fork; first done. iIntros "%nt %σ1 %κ %κs Hσ !>".
     iDestruct (gen_heap_valid with "Hσ Hl") as %Hlookup.
-    iSplit; first eauto with zoo. iIntros "%e2 %σ2 %es %ϕ %Hstep %Hϕ _ !> !>".
+    iSplit; first eauto with zoo. iIntros "%e2 %σ2 %es %Hstep _ !> !>".
     invert_base_step.
     iMod (gen_heap_update with "Hσ Hl") as "($ & Hl)".
     iFrame. iSteps.
@@ -233,27 +212,22 @@ Section zoo_G.
 
   Lemma base_reducible_cas l v v1 v2 σ :
     σ.(state_heap) !! l = Some v →
-    val_physical v →
-    val_physical v1 →
     base_reducible (Cas #l v1 v2) σ.
   Proof.
     intros.
     destruct
-      v as [[b | i | l' | |] | | [cid |] tag []],
-      v1 as [[b1 | i1 | l1 | |] | | [cid1 |] tag1 []].
+      v as [[b | i | l'] | | tag []],
+      v1 as [[b1 | i1 | l1] | | tag1 []].
     all:
       try first
       [ destruct (decide (b = b1)); first subst
       | destruct (decide (i = i1)); first subst
       | destruct (decide (l' = l1)); first subst
-      | destruct (decide (cid = cid1)); first subst
       | destruct (decide (tag = tag1)); first subst
       ].
     all: eauto with zoo.
   Qed.
   Lemma wp_cas l dq v v1 v2 E Φ :
-    val_physical v →
-    val_physical v1 →
     ▷ l ↦{dq} v -∗
     ▷ (
       ( ⌜val_neq v v1⌝ -∗
@@ -261,7 +235,6 @@ Section zoo_G.
         Φ #false
       ) ∧ (
         ⌜val_eq v v1⌝ -∗
-        ⌜val_consistency v v1⌝ -∗
         l ↦{dq} v -∗
           ⌜dq = DfracOwn 1⌝ ∗
           l ↦{dq} v ∗
@@ -272,21 +245,20 @@ Section zoo_G.
     ) -∗
     WP Cas #l v1 v2 @ E {{ Φ }}.
   Proof.
-    iIntros "% % >Hl HΦ".
-    iApply wp_lift_atomic_base_step_no_fork; first done. iIntros "%nt %σ1 %κ %κs (Hσ & Hκs) !>".
+    iIntros ">Hl HΦ".
+    iApply wp_lift_atomic_base_step_no_fork; first done. iIntros "%nt %σ1 %κ %κs Hσ !>".
     iDestruct (gen_heap_valid with "Hσ Hl") as %Hlookup.
 
     iSplit. { iPureIntro. eapply base_reducible_cas; done. }
-    iIntros "%e2 %σ2 %es %ϕ %Hstep %Hϕ _ !> !>".
+    iIntros "%e2 %σ2 %es %Hstep _ !> !>".
     destruct
-      v as [[b | i | l' | |] | | [cid |] tag []],
-      v1 as [[b1 | i1 | l1 | |] | | [cid1 |] tag1 []].
+      v as [[b | i | l'] | | tag []],
+      v1 as [[b1 | i1 | l1] | | tag1 []].
     all:
       try first
       [ destruct (decide (b = b1)); first subst
       | destruct (decide (i = i1)); first subst
       | destruct (decide (l' = l1)); first subst
-      | destruct (decide (cid = cid1)); first subst
       | destruct (decide (tag = tag1)); first subst
       ].
     all: invert_base_step; last try by exfalso.
@@ -298,15 +270,13 @@ Section zoo_G.
             iFrame; iSteps; naive_solver
         | context [true] =>
             iDestruct "HΦ" as "(_ & HΦ)";
-            iDestruct ("HΦ" with "[//] [//] Hl") as "(-> & Hl & HΦ)";
+            iDestruct ("HΦ" with "[//] Hl") as "(-> & Hl & HΦ)";
             iMod (gen_heap_update with "Hσ Hl") as "($ & Hl)";
             iFrame; iSteps; naive_solver
         end
       end.
   Qed.
   Lemma wp_cas_literal l dq lit lit1 v2 E Φ :
-    literal_physical lit →
-    literal_physical lit1 →
     ▷ l ↦{dq} #lit -∗
     ▷ (
       ( ⌜lit ≠ lit1⌝ -∗
@@ -324,16 +294,15 @@ Section zoo_G.
     ) -∗
     WP Cas #l #lit1 v2 @ E {{ Φ }}.
   Proof.
-    iIntros "% % >Hl HΦ".
+    iIntros ">Hl HΦ".
     iApply (wp_cas with "Hl"); [done.. |].
     iSplit.
     - iDestruct "HΦ" as "($ & _)".
     - iDestruct "HΦ" as "(_ & HΦ)".
-      iIntros "!> %Heq _".
+      iIntros "!> %Heq".
       iApply ("HΦ" with "[//]").
   Qed.
   Lemma wp_cas_suc l lit lit1 v2 E :
-    literal_physical lit →
     lit = lit1 →
     {{{
       ▷ l ↦ #lit
@@ -344,7 +313,7 @@ Section zoo_G.
       l ↦ v2
     }}}.
   Proof.
-    iIntros (Hlit ->) "%Φ >Hl HΦ".
+    iIntros (->) "%Φ >Hl HΦ".
     iApply (wp_cas_literal with "Hl"); [done.. |].
     iSteps.
   Qed.
@@ -360,9 +329,9 @@ Section zoo_G.
     }}}.
   Proof.
     iIntros "%Φ >Hl HΦ".
-    iApply wp_lift_atomic_base_step_no_fork; first done. iIntros "%nt %σ1 %κ %κs (Hσ & Hκs) !>".
+    iApply wp_lift_atomic_base_step_no_fork; first done. iIntros "%nt %σ1 %κ %κs Hσ !>".
     iDestruct (gen_heap_valid with "Hσ Hl") as %Hlookup.
-    iSplit; first eauto with zoo. iIntros "%e2 %σ2 %es %ϕ %Hstep %Hϕ _ !> !>".
+    iSplit; first eauto with zoo. iIntros "%e2 %σ2 %es %Hstep _ !> !>".
     invert_base_step.
     iMod (gen_heap_update with "Hσ Hl") as "($ & Hl)".
     iFrame. iSteps.
@@ -374,101 +343,9 @@ Section zoo_G.
     WP Fork e @ E {{ Φ }}.
   Proof.
     iIntros "H HΦ".
-    iApply wp_lift_atomic_base_step; first done. iIntros "%nt %σ1 %κ %κs (Hσ1 & Hκs) !>".
-    iSplit; first auto with zoo. iIntros "%v2 %σ2 %es %ϕ %Hstep %Hϕ _ !> !> !>".
+    iApply wp_lift_atomic_base_step; first done. iIntros "%nt %σ1 %κ %κs Hσ1 !>".
+    iSplit; first auto with zoo. iIntros "%v2 %σ2 %es %Hstep _ !> !> !>".
     invert_base_step.
     iFrame.
-  Qed.
-
-  Lemma wp_proph E :
-    {{{ True }}}
-      Proph @ E
-    {{{ prophs pid,
-      RET #pid;
-      prophet_model pid prophs
-    }}}.
-  Proof.
-    iIntros "%Φ _ HΦ".
-    iApply wp_lift_atomic_base_step_no_fork; first done. iIntros "%nt %σ1 %κ %κs (Hσ & Hκs) !>".
-    iSplit; first eauto with zoo. iIntros "%e2 %σ2 %es %ϕ %Hstep %Hϕ _ !> !>".
-    invert_base_step.
-    iMod (prophet_map_new pid with "Hκs") as "(Hκs & Hp)"; first done.
-    iFrame. iSteps.
-  Qed.
-
-  Lemma resolve_reducible e σ pid v :
-    Atomic e →
-    reducible e σ →
-    reducible (Resolve e #pid v) σ.
-  Proof.
-    intros A (κ & e' & σ' & es & ϕ & H).
-    exists (κ ++ [(pid, (default v (to_val e'), v))]), e', σ', es, ϕ.
-    eapply (Ectx_step []); try done.
-    assert (∃ w, Val w = e') as (w & <-).
-    { unfold Atomic in A. apply (A σ e' κ σ' es) in H. unfold is_Some in H.
-      destruct H as [w H]. exists w. simpl in H. apply (of_to_val _ _ H).
-    }
-    simpl. econstructor. apply prim_step_to_val_is_base_step. done.
-  Qed.
-  Lemma step_resolve e v1 v2 σ1 κ e2 σ2 es ϕ :
-    Atomic e →
-    prim_step (Resolve e v1 v2) σ1 κ e2 σ2 es ϕ →
-    base_step (Resolve e v1 v2) σ1 κ e2 σ2 es ϕ.
-  Proof.
-    intros A [K e1' e2' Hfill -> step]. simpl in *.
-    induction K as [| k K _] using rev_ind.
-    - simpl in *. subst. invert_base_step. constructor. done.
-    - rewrite fill_app /= in Hfill. destruct k; inversion Hfill; subst; clear Hfill.
-      + assert (fill_item k (fill K e1') = fill (K ++ [k]) e1') as Heq1; first by rewrite fill_app.
-        assert (fill_item k (fill K e2') = fill (K ++ [k]) e2') as Heq2; first by rewrite fill_app.
-        rewrite fill_app /=. rewrite Heq1 in A.
-        assert (is_Some (to_val (fill (K ++ [k]) e2'))) as H.
-        { eapply (A σ1 _ κ σ2 es), (Ectx_step (K ++ [k])); done. }
-        destruct H as [v H]. apply to_val_fill_some in H. destruct H, K; done.
-      + rename select (of_val v1 = _) into Hv1.
-        assert (to_val (fill K e1') = Some v1) as Hfill_v1 by rewrite -Hv1 //.
-        apply to_val_fill_some in Hfill_v1 as (-> & ->).
-        invert_base_step.
-      + rename select (of_val v2 = _) into Hv2.
-        assert (to_val (fill K e1') = Some v2) as Hfill_v2 by rewrite -Hv2 //.
-        apply to_val_fill_some in Hfill_v2 as (-> & ->).
-        invert_base_step.
-  Qed.
-  Lemma wp_resolve e pid v prophs E Φ :
-    Atomic e →
-    to_val e = None →
-    prophet_model pid prophs -∗
-    WP e @ E {{ res,
-      ∀ prophs',
-      ⌜prophs = (res, v) :: prophs'⌝ -∗
-      prophet_model pid prophs' -∗
-      Φ res
-    }} -∗
-    WP Resolve e #pid v @ E {{ Φ }}.
-  Proof.
-    iIntros "%Hatomic %He Hpid H".
-    rewrite !wp_unfold /wp_pre /= He. simpl in *.
-    iIntros "%nt %σ1 %κ %κs Hσ".
-    destruct κ as [| (pid' & (w' & v')) κ' _] using rev_ind.
-    - iMod ("H" with "Hσ") as "(%Hreducible & H)".
-      iSplitR. { iPureIntro. apply resolve_reducible; done. }
-      iIntros "!> %e2 %σ2 %es %ϕ %Hstep".
-      exfalso. apply step_resolve in Hstep; last done.
-      invert_base_step.
-      destruct κ; done.
-    - rewrite -assoc.
-      iMod ("H" with "Hσ") as "(%Hreducible & H)".
-      iSplitR. { iPureIntro. apply resolve_reducible; done. }
-      iIntros "!> %e2 %σ2 %es %ϕ %Hstep %HΦ H£".
-      apply step_resolve in Hstep; last done.
-      invert_base_step. simplify_list_eq.
-      iMod ("H" $! (Val w') σ2 es ϕ with "[%] [//] H£") as "H".
-      { eexists [] _ _; done. }
-      do 2 iModIntro.
-      iMod "H" as "(($ & Hκs) & H)".
-      iMod (prophet_map_resolve pid' (w', v') κs with "Hκs Hpid") as (vs' ->) "($ & Hpid')".
-      rewrite !wp_unfold /wp_pre /=.
-      iDestruct "H" as "(HΦ & $)".
-      iSteps.
   Qed.
 End zoo_G.
