theories/language/state_interp.v
@@ -5,8 +5,6 @@ From iris.base_logic Require Export
 
 From zoo Require Import
   prelude.
-From zoo.iris.base_logic Require Export
-  prophet_map.
 From zoo.iris.program_logic Require Export
   wp.
 From zoo.iris Require Import
@@ -22,13 +20,11 @@ Implicit Types κ : list observation.
 Class ZooGpre Σ := {
   #[global] zoo_Gpre_inv_Gpre :: invGpreS Σ ;
   #[local] zoo_Gpre_heap_Gpre :: gen_heapGpreS location val Σ ;
-  #[local] zoo_Gpre_prophecy_Gpre :: ProphetMapGpre Σ prophet_id (val * val) ;
 }.
 
 Definition zoo_Σ := #[
   invΣ ;
-  gen_heapΣ location val ;
-  prophet_map_Σ prophet_id (val * val)
+  gen_heapΣ location val
 ].
 #[global] Instance subG_zoo_Σ Σ :
   subG zoo_Σ Σ →
@@ -40,13 +36,11 @@ Qed.
 Class ZooG Σ := {
   zoo_G_inv_G : invGS Σ ;
   #[global] zoo_G_heap_G :: gen_heapGS location val Σ ;
-  #[global] zoo_G_prophecy_map_G :: ProphetMapG Σ prophet_id (val * val) ;
 }.
-#[global] Arguments Build_ZooG _ {_ _ _} : assert.
+#[global] Arguments Build_ZooG _ {_ _} : assert.
 
 Definition zoo_state_interp `{zoo_G : !ZooG Σ} (_ : nat) σ κ : iProp Σ :=
-  gen_heap_interp σ.(state_heap) ∗
-  prophet_map_interp κ σ.(state_prophets).
+  gen_heap_interp σ.(state_heap).
 #[global] Instance zoo_G_iris_G `{zoo_G : !ZooG Σ} : IrisG zoo Σ := {
   iris_G_inv_G :=
     zoo_G_inv_G ;
@@ -62,7 +56,6 @@ Lemma zoo_init `{zoo_Gpre : !ZooGpre Σ} `{inv_G : !invGS Σ} nt σ κ :
     state_interp nt σ κ.
 Proof.
   iMod (gen_heap_init σ.(state_heap)) as (?) "(Hσ & _)".
-  iMod (prophet_map_init κ σ.(state_prophets)) as "(% & Hκ)".
   iExists (Build_ZooG Σ). iFrame. iSteps.
 Qed.
 Lemma zoo_init' `{zoo_Gpre : !ZooGpre Σ} `{inv_G : !invGS Σ} σ κ :
