theories/language/tactics.v
@@ -11,109 +11,91 @@ From zoo Require Import
 Create HintDb zoo.
 
 Ltac reshape_expr e tac :=
-  let rec go K prophs e :=
+  let rec go K e :=
     match e with
     | _ =>
-        lazymatch prophs with
-        | nil =>
-            tac K e
-        | _ =>
-            fail
-        end
+        tac K e
     | App ?e1 (Val ?v2) =>
-        add_ectxi (CtxApp1 v2) K prophs e1
+        add_ectxi (CtxApp1 v2) K e1
     | App ?e1 ?e2 =>
-        add_ectxi (CtxApp2 e1) K prophs e2
+        add_ectxi (CtxApp2 e1) K e2
     | Unop ?op ?e =>
-        add_ectxi (CtxUnop op) K prophs e
+        add_ectxi (CtxUnop op) K e
     | Binop ?op ?e1 (Val ?v2) =>
-        add_ectxi (CtxBinop1 op v2) K prophs e1
+        add_ectxi (CtxBinop1 op v2) K e1
     | Binop ?op ?e1 ?e2 =>
-        add_ectxi (CtxBinop2 op e1) K prophs e2
+        add_ectxi (CtxBinop2 op e1) K e2
     | Equal ?e1 (Val ?v2) =>
-        add_ectxi (CtxEqual1 v2) K prophs e1
+        add_ectxi (CtxEqual1 v2) K e1
     | Equal ?e1 ?e2 =>
-        add_ectxi (CtxEqual2 e1) K prophs e2
+        add_ectxi (CtxEqual2 e1) K e2
     | If ?e0 ?e1 ?e2 =>
-        add_ectxi (CtxIf e1 e2) K prophs e0
+        add_ectxi (CtxIf e1 e2) K e0
     | Constr ?tag ?es =>
-        go_list K prophs (CtxConstr tag) es
+        go_list K (CtxConstr tag) es
     | Proj ?proj ?e =>
-        add_ectxi (CtxProj proj) K prophs e
+        add_ectxi (CtxProj proj) K e
     | Match ?e0 ?x ?e1 ?brs =>
-        add_ectxi (CtxMatch x e1 brs) K prophs e0
-    | Reveal ?e =>
-        add_ectxi CtxReveal K prophs e
+        add_ectxi (CtxMatch x e1 brs) K e0
     | For (Val ?v1) ?e2 ?e3 =>
-        add_ectxi (CtxFor2 v1 e3) K prophs e2
+        add_ectxi (CtxFor2 v1 e3) K e2
     | For ?e1 ?e2 ?e3 =>
-        add_ectxi (CtxFor1 e2 e3) K prophs e1
+        add_ectxi (CtxFor1 e2 e3) K e1
     | Record ?es =>
-        go_list K prophs CtxRecord es
+        go_list K CtxRecord es
     | Alloc ?e1 (Val ?v2) =>
-        add_ectxi (CtxAlloc1 v2) K prophs e1
+        add_ectxi (CtxAlloc1 v2) K e1
     | Alloc ?e1 ?e2 =>
-        add_ectxi (CtxAlloc2 e1) K prophs e2
+        add_ectxi (CtxAlloc2 e1) K e2
     | Load ?e =>
-        add_ectxi CtxLoad K prophs e
+        add_ectxi CtxLoad K e
     | Store ?e1 (Val ?v2) =>
-        add_ectxi (CtxStore1 v2) K prophs e1
+        add_ectxi (CtxStore1 v2) K e1
     | Store ?e1 ?e2 =>
-        add_ectxi (CtxStore2 e1) K prophs e2
+        add_ectxi (CtxStore2 e1) K e2
     | Xchg ?e1 (Val ?v2) =>
-        add_ectxi (CtxXchg1 v2) K prophs e1
+        add_ectxi (CtxXchg1 v2) K e1
     | Xchg ?e1 ?e2 =>
-        add_ectxi (CtxXchg2 e1) K prophs e2
+        add_ectxi (CtxXchg2 e1) K e2
     | Cas ?e0 (Val ?v1) (Val ?v2) =>
-        add_ectxi (CtxCas0 v1 v2) K prophs e0
+        add_ectxi (CtxCas0 v1 v2) K e0
     | Cas ?e0 ?e1 (Val ?v2) =>
-        add_ectxi (CtxCas1 e0 v2) K prophs e1
+        add_ectxi (CtxCas1 e0 v2) K e1
     | Cas ?e0 ?e1 ?e2 =>
-        add_ectxi (CtxCas2 e0 e1) K prophs e2
+        add_ectxi (CtxCas2 e0 e1) K e2
     | Faa ?e1 (Val ?v2) =>
-        add_ectxi (CtxFaa1 v2) K prophs e1
+        add_ectxi (CtxFaa1 v2) K e1
     | Faa ?e1 ?e2 =>
-        add_ectxi (CtxFaa2 e1) K prophs e2
-    | Resolve ?e0 (Val ?v1) (Val ?v2) =>
-        go K (cons (v1, v2) prophs) e0
-    | Resolve ?e0 ?e1 (Val ?v2) =>
-        add_ectxi (CtxResolve1 e0 v2) K prophs e1
-    | Resolve ?e0 ?e1 ?e2 =>
-        add_ectxi (CtxResolve2 e0 e1) K prophs e2
+        add_ectxi (CtxFaa2 e1) K e2
     end
-  with go_list K prophs ctx es :=
-    go_list' K prophs ctx (@nil val) es
-  with go_list' K prophs ctx vs es :=
+  with go_list K ctx es :=
+    go_list' K ctx (@nil val) es
+  with go_list' K ctx vs es :=
     lazymatch es with
     | cons ?e ?es =>
         lazymatch e with
         | Val ?v =>
-            go_list' K prophs ctx (cons v vs) es
+            go_list' K ctx (cons v vs) es
         | _ =>
-            go_list'' K prophs ctx vs e es
+            go_list'' K ctx vs e es
         end
     | _ =>
         fail
     end
-  with go_list'' K prophs ctx vs e es :=
+  with go_list'' K ctx vs e es :=
     first
-    [ add_ectxi (ctx (rev vs) es) K prophs e
+    [ add_ectxi (ctx (rev vs) es) K e
     | lazymatch vs with
       | nil =>
           fail
       | cons ?v ?vs =>
-          go_list'' K prophs ctx vs (Val v) (cons e es)
+          go_list'' K ctx vs (Val v) (cons e es)
       end
     ]
-  with add_ectxi k K prophs e :=
-    lazymatch prophs with
-    | nil =>
-        go (cons k K) (@nil (val * val)) e
-    | cons (?v1, ?v2) ?prophs =>
-        add_ectxi (CtxResolve0 k v1 v2) K prophs e
-    end
+  with add_ectxi k K e :=
+    go (cons k K) e
   in
-  go (@nil ectxi) (@nil (val * val)) e.
+  go (@nil ectxi) e.
 
 Ltac invert_base_step :=
   repeat match goal with
@@ -121,7 +103,7 @@ Ltac invert_base_step :=
       progress simplify_map_eq/=
   | H: to_val _ = Some _ |- _ =>
       apply of_to_val in H
-  | H: base_step ?e _ _ _ _ _ _ |- _ =>
+  | H: base_step ?e _ _ _ _ _ |- _ =>
      try (is_var e; fail 1);
      invert H
   end.
@@ -140,56 +122,46 @@ Ltac invert_base_step :=
 #[global] Hint Extern 0 (
   base_reducible _ _
 ) =>
-  do 5 eexists; simpl
+  do 4 eexists; simpl
 : zoo.
 #[global] Hint Extern 0 (
   base_reducible_no_obs _ _
 ) =>
-  do 4 eexists; simpl
+  do 3 eexists; simpl
 : zoo.
 
 #[global] Hint Extern 1 (
-  base_step _ _ _ _ _ _ _
+  base_step _ _ _ _ _ _
 ) =>
   econstructor
 : zoo.
 #[global] Hint Extern 0 (
-  base_step (Equal _ _) _ _ _ _ _ _
+  base_step (Equal _ _) _ _ _ _ _
 ) =>
   eapply base_step_equal_fail; simpl; [| | try injection]
 : zoo.
 #[global] Hint Extern 0 (
-  base_step (Equal _ _) _ _ _ _ _ _
+  base_step (Equal _ _) _ _ _ _ _
 ) =>
   eapply base_step_equal_suc; simpl
 : zoo.
 #[global] Hint Extern 0 (
-  base_step (Reveal _) _ _ _ _ _ _
-) =>
-  eapply base_step_reveal'
-: zoo.
-#[global] Hint Extern 0 (
-  base_step (Record _) _ _ _ _ _ _
+  base_step (Record _) _ _ _ _ _
 ) =>
   eapply base_step_record'
 : zoo.
 #[global] Hint Extern 0 (
-  base_step (Alloc _ _) _ _ _ _ _ _
+  base_step (Alloc _ _) _ _ _ _ _
 ) =>
   apply base_step_alloc'
 : zoo.
 #[global] Hint Extern 0 (
-  base_step (Cas _ _ _) _ _ _ _ _ _
+  base_step (Cas _ _ _) _ _ _ _ _
 ) =>
   eapply base_step_cas_fail; simpl; [| | | try injection]
 : zoo.
 #[global] Hint Extern 0 (
-  base_step (Cas _ _ _) _ _ _ _ _ _
+  base_step (Cas _ _ _) _ _ _ _ _
 ) =>
   eapply base_step_cas_suc; simpl
-: zoo.
-#[global] Hint Extern 0 (
-  base_step Proph _ _ _ _ _ _
-) =>
-  apply base_step_proph'
 : zoo.
