theories/language/typeclass_instances.v
@@ -64,13 +64,8 @@ Section atomic.
     solve_atomic.
   Qed.
 
-  #[global] Instance proj_atomic proj cid tag vs :
-    Atomic (Proj proj $ Val $ ValConstr cid tag vs).
-  Proof.
-    solve_atomic.
-  Qed.
-  #[global] Instance reveal_atomic cid tag vs :
-    Atomic (Reveal $ Val $ ValConstr cid tag vs).
+  #[global] Instance proj_atomic proj tag vs :
+    Atomic (Proj proj $ Val $ ValConstr tag vs).
   Proof.
     solve_atomic.
   Qed.
@@ -119,37 +114,6 @@ Section atomic.
     Atomic Yield.
   Proof.
     solve_atomic.
-  Qed.
-
-  #[global] Instance proph_atomic :
-    Atomic Proph.
-  Proof.
-    solve_atomic.
-  Qed.
-  #[global] Instance resolve_atomic e v1 v2 :
-    Atomic e →
-    Atomic (Resolve e (Val v1) (Val v2)).
-  Proof.
-    rename e into e1. intros H σ1 e2 κ σ2 es ϕ [K e1' e2' Hfill -> Hstep].
-    simpl in *. induction K as [| k K _] using rev_ind; simpl in Hfill.
-    - subst. inversion_clear Hstep.
-      eapply (H σ1 (Val _) _ σ2 es), base_prim_step. done.
-    - rewrite fill_app. rewrite fill_app in Hfill.
-      assert (∀ v, Val v = fill K e1' → False) as Hfill_absurd.
-      { intros v Hv.
-        assert (to_val (fill K e1') = Some v) as Htv by by rewrite -Hv.
-        apply to_val_fill_some in Htv. destruct Htv as [-> ->]. inversion Hstep.
-      }
-      destruct k; (
-        inversion Hfill; clear Hfill; subst;
-        try match goal with H : Val ?v = fill K e1' |- _ =>
-          apply Hfill_absurd in H; done
-        end
-      ).
-      refine (_ (H σ1 (fill (K ++ [_]) e2') _ σ2 es _ _)).
-      + intro Hs. simpl in *.
-        destruct Hs as [v Hs]. apply to_val_fill_some in Hs. destruct Hs, K; done.
-      + econstructor; try done. simpl. by rewrite fill_app.
   Qed.
 End atomic.
 
@@ -276,7 +240,7 @@ Section pure_exec.
     PureExec
       True
       1
-      (Equal (Val $ ValConstr None tag1 []) (Val $ ValConstr None tag2 []))
+      (Equal (Val $ ValConstr tag1 []) (Val $ ValConstr tag2 []))
       (Val $ ValBool (bool_decide (tag1 = tag2))).
   Proof.
     solve_pure_exec.
@@ -285,7 +249,7 @@ Section pure_exec.
     PureExec
       True
       1
-      (Equal (Val $ ValConstr None tag1 []) (Val $ ValConstr None tag2 (v2 :: vs2)))
+      (Equal (Val $ ValConstr tag1 []) (Val $ ValConstr tag2 (v2 :: vs2)))
       (Val $ ValBool false).
   Proof.
     solve_pure_exec.
@@ -294,7 +258,7 @@ Section pure_exec.
     PureExec
       True
       1
-      (Equal (Val $ ValConstr None tag1 (v1 :: vs1)) (Val $ ValConstr None tag2 []))
+      (Equal (Val $ ValConstr tag1 (v1 :: vs1)) (Val $ ValConstr tag2 []))
       (Val $ ValBool false).
   Proof.
     solve_pure_exec.
@@ -324,27 +288,27 @@ Section pure_exec.
       (to_vals es = Some vs)
       1
       (Constr tag es)
-      (Val $ ValConstr None tag vs).
+      (Val $ ValConstr tag vs).
   Proof.
     intros <-%of_to_vals.
     apply nsteps_once, pure_base_step_pure_step.
     split; [solve_exec_safe | solve_exec_puredet].
   Qed.
-  #[global] Instance pure_proj proj cid tag vs v :
+  #[global] Instance pure_proj proj tag vs v :
     PureExec
       (vs !! proj = Some v)
       1
-      (Proj proj $ Val $ ValConstr cid tag vs)
+      (Proj proj $ Val $ ValConstr tag vs)
       (Val v).
   Proof.
     solve_pure_exec.
   Qed.
-  #[global] Instance pure_match cid tag vs x e brs :
+  #[global] Instance pure_match tag vs x e brs :
     PureExec
       True
       1
-      (Match (Val $ ValConstr cid tag vs) x e brs)
-      (match_apply cid tag vs x e brs).
+      (Match (Val $ ValConstr tag vs) x e brs)
+      (match_apply tag vs x e brs).
   Proof.
     solve_pure_exec.
   Qed.
